
  {
    "@context": {
      "rdf": "http://www.w3.org/1999/02/22-rdf-syntax-ns#",
      "rdfs": "http://www.w3.org/2000/01/rdf-schema#",
      "dt4be": "https://github.com/PeterInfraBIM/DigitalTwin4BuiltEnvironment/blob/main/schema.jsonld#",
      "schema": "http://schema.org/",
      "xsd": "http://www.w3.org/2001/XMLSchema#"
      }
  },
  {
    "@id": "dt4be:Building",
    "@type": "rdfs:Class",
    "rdfs:comment": "A building represents a structure that provides shelter for its occupants or contents and stands in one place. The building is also used to provide a basic element within the spatial structure hierarchy for the components of a building project (together with site, storey, and space).",
    "rdfs:label": "Building"
  },
  {
    "@id": "dt4be:elevationOfRefHeight",
    "@type": "rdf:Property",
    "rdfs:label": "elevationOfRefHeight",
    "rdfs:comment": "Elevation above sea level of the reference height used for all storey elevation measures, equals to height 0.0. It is usually the ground floor level.",
    "rdfs:domain": {
        "@id": "dt4be:Building"
      },
    "rdfs:range": {
        "@id": "xsd:float"
      }
  },
  {
    "@id": "dt4be:elevationOfTerrain",
    "@type": "rdf:Property",
    "rdfs:label": "elevationOfTerrain",
    "rdfs:comment": "Elevation above the minimal terrain level around the foot print of the building, given in elevation above sea level.",
    "rdfs:domain": {
        "@id": "dt4be:Building"
      },
    "rdfs:range": {
        "@id": "xsd:float"
      }
   }

